towards lower-level networking callbacks

src/tls/Transport.fst
@@ -10,34 +10,71 @@ open FStar.Bytes
 open FStar.Error
 open TLSError
 
-// make this type abstract?
 
-type external = FStar.Dyn.dyn
+/// 18-01-23 We now have function pointers matching the types used in
+/// mitls.h. After hoisting for Kremlin extraction, we treat the
+/// explicit context as a dyn to avoid climbing in universes.
+
+type pvoid = FStar.Dyn.dyn
+type size_t = UInt32.t 
+type pfn_send = 
+  pvoid -> 
+  output_buffer: FStar.Buffer.buffer UInt8.t -> 
+  max_len: size_t -> ST Int32.t
+  (requires fun h0 -> 
+    Buffer.live h0 output_buffer /\ 
+    UInt32.v max_len = Buffer.length output_buffer)
+  (ensures fun h0 r h1 -> 
+    let v = Int32.v r in
+    modifies_none h0 h1 /\
+    (v = -1 \/ (0 <= v /\ v <= UInt32.v max_len)))
+
+type pfn_recv = 
+  pvoid -> 
+  input_buffer: FStar.Buffer.buffer UInt8.t -> 
+  max_len: size_t -> ST Int32.t
+  (requires fun h0 ->
+    Buffer.live h0 input_buffer /\
+    UInt32.v max_len = Buffer.length input_buffer)
+  (ensures fun h0 r h1 -> 
+    let v = Int32.v r in 
+    Buffer.modifies_1 input_buffer h0 h1 /\ 
+    (v = -1 \/ (0 <= v /\ v <= UInt32.v max_len)))
+    
 noeq type t = {
-  app_context : external;
-  snd: external -> bytes -> ST (optResult string unit) (fun _ -> True) (fun h0 _ h1 -> h0 == h1);
-  rcv: external  -> max:nat -> ST (recv_result max) (fun _ -> True) (fun h0 _ h1 -> h0 == h1) }
+  ptr : pvoid;
+  snd: pfn_send;
+  rcv: pfn_recv }
 
-let callbacks v send recv = { app_context = v; snd = send; rcv = recv }
+let callbacks v send recv: t = { ptr = v; snd = send; rcv = recv }
 
-// platform implementation
+/// 18-01-23 FStar.Tcp implementation. We now have to coerce
+/// FStar.Tcp.networkStream to dyn and back when using TCP instead of
+/// C-defined callbacks, and to bridge the Low*/F* calling conventions.
 
-/// 18-01-23 after hoisting for Kremlin extraction, we treat the
-/// explicit context as a dyn to avoid climbing in universes; this
-/// forces us to coerce FStar.Tcp.networkStream to dyn and back when
-/// using TCP instead of C-defined callbacks. Any better idea?
+//#set-options "--lax" 
+private val send_tcp: pfn_send
+let send_tcp ptr buffer len =
+  let n: networkStream = FStar.Dyn.undyn ptr in
+  let v = BufferBytes.to_bytes (UInt32.v len) buffer in 
+  match send n v with 
+  | Correct () -> Int.Cast.uint32_to_int32 len
+  | Error _ignored -> -1l
 
-#set-options "--lax" 
-private let send_tcp (x:external) (b:bytes): ST (optResult string unit) (fun _ -> True) (fun h0 _ h1 -> h0 == h1) = 
-  let n: networkStream = FStar.Dyn.undyn x in
-  send n b
-private let recv_tcp (x:external) (max:nat): ST (recv_result max) (fun _ -> True) (fun h0 _ h1 -> h0 == h1) = 
-  let n: networkStream = FStar.Dyn.undyn x in
-  recv_async n max
-#reset-options
+private val recv_tcp: pfn_recv 
+let recv_tcp ptr buffer len = 
+  let n: networkStream = FStar.Dyn.undyn ptr in
+  match recv_async n (UInt32.v len) with 
+  | RecvWouldBlock -> 0l // return instead EAGAIN or EWOULDBLOCK?
+  | RecvError _ignored -> -1l 
+  | Received b -> 
+    let target = Buffer.sub buffer 0ul (Bytes.len b) in
+    BufferBytes.store_bytes (length b) target 0 b;
+    Int.Cast.uint32_to_int32 (Bytes.len b)
+//#reset-options
 
+let wrap tcp: Dv t = callbacks (FStar.Dyn.mkdyn tcp) send_tcp recv_tcp
 
-let wrap tcp: t = callbacks (FStar.Dyn.mkdyn tcp) send_tcp recv_tcp
 type tcpListener = tcpListener
 
 let listen domain port : ML tcpListener = listen domain port
@@ -47,19 +84,19 @@ let close = close
 
 // following the indirection
 
-let send tcp data = tcp.snd tcp.v data
-let recv tcp len = tcp.rcv tcp.v len
+let send tcp buffer len = tcp.snd tcp.ptr buffer len 
+let recv tcp buffer len = tcp.rcv tcp.ptr buffer len 
 
-val test: t networkStream -> bytes -> ML unit
-let test (tcp:t networkStream) (data:bytes) = 
-  let h0 = FStar.HyperStack.ST.get() in 
-  let _ = tcp.snd tcp.v data in
-  let h1 = FStar.HyperStack.ST.get() in 
-  assert (h0==h1)
-
+val test: t -> b: Buffer.buffer UInt8.t {Buffer.length b = 5} -> ST unit
+  (requires fun h0 -> Buffer.live h0 b)
+  (ensures fun h0 r h1 -> h0 == h1)
+let test tcp b =
+  let _ = send tcp b 5ul in
+  ()
 
 // for now we get a runtime error in case of partial write on an asynchronous socket
 
+(* 18-01-23 not used in quic2c? 
 
 // forces read to complete, even if the socket is non-blocking.
 // this may cause spinning.
@@ -80,3 +117,4 @@ let rec really_read_rec prev tcp len =
       | RecvError e -> RecvError e
 
 let really_read = really_read_rec empty_bytes
+*)
